Direct bigstep semantics for Lua (not using LIR)

lua.v
@@ -12,6 +12,7 @@ Require Import LIR.maps.
 Require Import LIR.pallene.
 Require Import LIR.lir.
 Require Import LIR.dyn.
+Require Import LIR.biglir.
 
 
 Inductive LE : Set :=
@@ -61,6 +62,12 @@ Fixpoint Lua2Lir (e : LE) : IRE :=
       IREBox TgFun (IREFun (IRELamb var IRTStar (Lua2Lir body)))
   | LEApp e1 e2 => IREFunApp (IREUnbox TgFun (Lua2Lir e1)) (Lua2Lir e2)
   end.
+
+
+Lemma LuaIsDyn : forall e, Lua2Lir e = dyn (Lua2Lir e).
+Proof.
+  induction e; simpl; congruence.
+Qed.
 
 
 Inductive LMem : Set :=
@@ -121,12 +128,165 @@ Inductive LValue : LE -> Prop :=
 | LVnil : LValue LENil
 | LVnum : forall n, LValue (LENum n)
 | LVtbl : forall a, LValue (LEAddr a)
-| LVfun : forall var e, LValue (LEFun var e)
+| LVfun : forall var body, LValue (LEFun var body)
 .
 
 
-(* Issues: 1. globals; 2. type of assignments *)
-Lemma Lua2LirTypeAux : forall Γ e, LEWT Γ e -> Γ |= Lua2Lir e : IRTStar.
+Reserved Notation "m '/' e ==> m1 '/' e1"
+(at level 40, e at level 39, m1 at level 39, e1 at level 39).
+
+Inductive Lstep : LMem -> LE -> LMem -> LE -> Prop :=
+| LStValue : forall m e, LValue e -> m / e ==> m / e
+| LStPlus : forall m e1 e2 m' n1 m'' n2,
+    m / e1 ==> m' / (LENum n1) ->
+    m' / e2 ==> m'' / (LENum n2) ->
+    m / LEPlus e1 e2 ==> m'' / LENum (n1 + n2)
+| LStCstr : forall m m' free,
+    (free, m') = Lfresh m ->
+    m / LECnst ==> m' / LEAddr free
+| LStGet : forall m e1 m' a e2 m'' idx,
+    m / e1 ==> m' / LEAddr a ->
+    m' / e2 ==> m'' / idx ->
+    m / LEGet e1 e2 ==> m'' / Lquery a idx m''
+| LStSet : forall m e1 m' a e2 m'' idx e3 v m''',
+    m / e1 ==> m' / LEAddr a ->
+    m' / e2 ==> m'' / idx ->
+    m'' / e3 ==> m''' / v ->
+    m / LESet e1 e2 e3 ==> LUpdate a idx v m''' / v
+| LStApp : forall m e1 var body e2 m' m'' v m''' res,
+     m / e1 ==> m' / LEFun var body ->
+     m' / e2 ==> m'' / v ->
+     m'' / ([var := v] body) ==> m''' / res ->
+     m / LEApp e1 e2 ==> m''' / res
+
+where "m / e ==> m1 / e1" := (Lstep m e m1 e1)
+.
+
+Example L1 : LEmptyMem / LEPlus (LENum 3) (LENum 5) ==>
+             LEmptyMem / LENum 8.
+Proof.
+  replace 8 with (3 + 5) by lia.
+  eauto using Lstep, LValue.
+Qed.
+
+
+Example L2 : LEmptyMem / LEApp (LEFun "x" (LEVar "x")) (LENum 10) ==>
+             LEmptyMem / LENum 10.
+Proof. eauto using Lstep, LValue. Qed.
+
+
+Lemma L2LirValue : forall e, LValue e -> Value (Lua2Lir e).
+Proof.
+  intros e HV.
+  inversion HV; simpl; subst; eauto using Value.
+Qed.
+
+
+Definition Lmem_correct (m : LMem) := forall a n,
+    LValue (Lquery a n m) /\ LEWT MEmpty (Lquery a n m).
+
+
+Lemma Lmem_correct_update : forall m a idx e,
+  Lmem_correct m -> LEWT MEmpty e -> LValue e ->
+     Lmem_correct (LUpdate a idx e m).
+Proof.
+  unfold Lmem_correct.
+  intros.
+  split;
+  simpl;
+    destruct (Nat.eq_dec a0 a); destruct (Index_dec n idx); subst; auto;
+    apply H.
+Qed.
+
+
+Lemma mem_correct_fresh : forall m m' free,
+  Lmem_correct m -> (free,m') = Lfresh m -> Lmem_correct m'.
+Proof.
+  unfold Lfresh. intros m m' free Hmc Heq. inversion Heq.
+  eauto using Lmem_correct_update,LValue,LEWT.
+Qed.
+
+
+Lemma LMCquery : forall a v m, Lmem_correct m -> LValue (Lquery a v m).
+Proof. intros a v m H. apply H. Qed.
+
+
+Lemma LMCWT : forall a v m, Lmem_correct m -> LEWT MEmpty (Lquery a v m).
+Proof. intros a v m H. apply H. Qed.
+
+
+Lemma inclusion_WT : forall Γ Γ' e,
+  inclusion Γ Γ' -> LEWT Γ e -> LEWT Γ' e.
+Proof.
+  intros Γ Γ' e Hin Hty.
+  generalize dependent Γ'.
+  induction Hty; eauto using LEWT, inclusion_update.
+Qed.
+
+
+Corollary WT_empty : forall Γ e, LEWT MEmpty e -> LEWT Γ e.
+Proof.
+  eauto using inclusion_WT, inclusion_empty.
+Qed.
+
+
+Lemma subst_WT : forall e2 Γ var e1,
+  LEWT (var |=> IRTStar; Γ) e2 -> LEWT MEmpty e1 -> LEWT Γ ([var := e1] e2).
+Proof.
+  induction e2; intros Γ var e1 HWT2 HWT1; simpl;
+  inversion HWT2; subst; eauto using LEWT.
+  - destruct (string_dec var s); eauto using WT_empty, InNotEq, LEWT.
+  - destruct (string_dec var s); subst.
+    + eauto using inclusion_WT, inclusion_shadow, LEWT.
+    + eauto using inclusion_WT, inclusion_permute, LEWT.
+Qed.
+
+
+Lemma luaPreservation : forall e m v m',
+  Lmem_correct m ->
+  LEWT MEmpty e ->
+  m / e ==> m' / v ->
+  Lmem_correct m' /\ LValue v /\ LEWT MEmpty v.
+Proof.
+  intros e m v m' HM HWT HSt.
+  induction HSt; inversion HWT; subst; repeat split;
+  try apply HM; eauto using LValue;
+  (* instantiate and split induction hyphoteses *)
+  repeat match goal with
+  | [ HM: Lmem_correct ?M,
+    HWT: LEWT MEmpty ?E,
+    IH: Lmem_correct ?M -> LEWT MEmpty ?E -> _ |- _ ] =>
+     specialize (IH HM HWT) as [? [? ?]]
+  end;
+  eauto using LValue, LEWT;
+  try match goal with
+  | [ HM: Lmem_correct ?M,
+      HFr: _ = Lfresh ?M |- _ ] =>
+     specialize (mem_correct_fresh _ _ _ HM HFr); clear HFr; intros
+  end;
+  eauto using LValue, LEWT,Lmem_correct_update, LMCquery, LMCWT,
+              Lmem_correct_update.
+  - inversion H1; subst.
+    apply LMCquery. apply IHHSt3;
+    eauto using subst_WT.
+  - inversion H1; subst.
+    apply LMCWT. eapply IHHSt3; eauto using subst_WT.
+  - inversion H1; subst.
+    eapply IHHSt3; eauto using subst_WT.
+  - inversion H1; subst.
+    eapply IHHSt3; eauto using subst_WT.
+Qed.
+
+
+Fixpoint MLua2Lir (m : LMem) : Mem :=
+  match m with
+  | LEmptyMem => EmptyMem
+  | LUpdate a n e m => Update a n (Lua2Lir e) (MLua2Lir m)
+  end.
+
+
+Lemma Lua2LirTypeAux : forall Γ e,
+  LEWT Γ e -> Γ |= Lua2Lir e : IRTStar.
 Proof.
   intros Γ e.
   generalize dependent Γ.
@@ -135,16 +295,100 @@ Proof.
 Qed.
 
 
-Lemma LuaIsDyn : forall e, Lua2Lir e = dyn (Lua2Lir e).
+Corollary Lua2LirType : forall e,
+    LEWT MEmpty e ->  MEmpty |= Lua2Lir e : IRTStar.
+Proof. eapply Lua2LirTypeAux. Qed.
+
+
+Lemma L2LirQuery : forall mem a idx,
+    Lua2Lir (Lquery a idx mem) =
+    query a (Lua2Lir idx) (MLua2Lir mem).
 Proof.
-  intros e.
-  induction e; simpl; try congruence.
+  intros mem a idx.
+  induction mem.
+  - simpl. trivial.
+  - simpl. destruct (Nat.eq_dec a a0); subst; trivial.
+    rewrite <- LuaIndex. destruct (Index_dec idx i); subst; trivial.
 Qed.
 
 
-Corollary Lua2LirType : forall e,
-    LEWT MEmpty e -> MEmpty |= Lua2Lir e : IRTStar.
-Proof. intros e. eapply Lua2LirTypeAux. Qed.
+Lemma L2LirFreshaux : forall m, Lfreshaux m = freshaux (MLua2Lir m).
+Proof. induction m; simpl; congruence. Qed.
+
+
+Lemma L2LirFresh : forall free m m',
+  (free, m') = Lfresh m -> (free, MLua2Lir m') = fresh (MLua2Lir m).
+Proof.
+  intros free m m' H.
+  unfold Lfresh in H. inversion H; subst.
+  unfold fresh. f_equal.
+  - apply L2LirFreshaux.
+  - rewrite LuaIndex. rewrite L2LirFreshaux. trivial.
+Qed.
+
+
+Lemma L2LirSubst : forall e1 var e2,
+  Lua2Lir (substitution var e1 e2) =
+  lir.substitution var (Lua2Lir e1) (Lua2Lir e2).
+Proof.
+  intros e1 var e2.
+  induction e2; simpl; try congruence.
+  - destruct (string_dec var s).
+    + destruct (string_dec s s); easy.
+    + destruct (string_dec s var); easy.
+  - destruct (string_dec var s); simpl; congruence.
+Qed.
+
+
+(* Propagate 'Lmem_correct' to all memories *)
+Ltac LmemC :=
+  match goal with
+    | [ M : LMem |- _] =>  (* for all memories *)
+      match goal with
+      | [ H : Lmem_correct M |- _] => fail 1  (* already done *)
+      | [ HSt: Lstep _ ?E M _ |- _] =>  (* else *)
+         assert(Lmem_correct M) by (eapply (luaPreservation E); eauto)
+      end
+    end.
+
+
+Theorem SymLua : forall e m v m',
+    Lmem_correct m ->
+    LEWT MEmpty e ->
+    m /e ==> m' / v  ->
+    bigStep (MLua2Lir m) (Lua2Lir e)
+            (MLua2Lir m') (Some (Lua2Lir v)).
+Proof.
+  intros e m v m' HMC HWT HSt.
+  induction HSt; inversion HWT; subst;
+  repeat LmemC;
+  eauto using bigStep, L2LirValue, L2LirFresh, L2LirQuery.
+  - simpl. apply BStBox.
+    eapply BStPlus.
+    + eapply BStUnbox.
+      replace (IREBox TgInt (IRENum n1)) with (Lua2Lir (LENum n1))
+        by trivial.
+      eapply IHHSt1; trivial.
+    + eapply BStUnbox.
+      replace (IREBox TgInt (IRENum n2)) with (Lua2Lir (LENum n2))
+        by trivial.
+      eapply IHHSt2; trivial.
+  - simpl. rewrite LuaIndex.
+    eapply BStSet; eauto.
+    eapply BStUnbox.
+    replace (IREBox TgTbl (IREAddr a)) with (Lua2Lir (LEAddr a))
+      by trivial. eauto.
+  - simpl. eapply BStFunapp; eauto.
+    eapply BStUnbox.
+    specialize (IHHSt1 HMC H2). eapply IHHSt1.
+    fold Lua2Lir. rewrite <- L2LirSubst.
+    eapply IHHSt3; eauto.
+     assert (LEWT MEmpty (LEFun var body)).
+     { eapply (luaPreservation e1 m); eauto. }
+     inversion H1; subst.
+     eapply subst_WT; eauto.
+     eapply (luaPreservation e2 m'); eauto.
+Qed.
 
 
 Fixpoint Pall2Lua (e : PE) : LE :=
@@ -160,4 +404,5 @@ Fixpoint Pall2Lua (e : PE) : LE :=
   | PEFun var _ e => LEFun var (Pall2Lua e)
   | PECast e _ => Pall2Lua e
   end.
+
 
